WIP WP rule for EStoreId

theories/rules/rules_EStoreId.v
@@ -1,7 +1,7 @@
 From iris.base_logic Require Export invariants gen_heap.
 From iris.program_logic Require Export weakestpre ectx_lifting.
 From iris.proofmode Require Import proofmode.
-From iris.algebra Require Import frac.
+From iris.algebra Require Import frac gmap.
 From cap_machine Require Export rules_base.
 
 Section cap_lang_rules.
@@ -18,34 +18,79 @@ Section cap_lang_rules.
   Implicit Types mem : Mem.
   Implicit Types lmem : LMem.
 
-  (* TODO @Denis *)
-  Lemma wp_estoreid E pc_p pc_b pc_e pc_a pc_v lw dst src :
-    decodeInstrWL lw = EStoreId dst src →
-    isCorrectLPC (LCap pc_p pc_b pc_e pc_a pc_v) →
+  Inductive EStoreId_spec : cap_lang.val -> Prop :=
+  | EStoreId_spec_success:
+    EStoreId_spec NextIV
+  |EStoreId_spec_failure:
+    EStoreId_spec FailedV.
 
-    {{{ PC ↦ᵣ LCap pc_p pc_b pc_e pc_a pc_v ∗ (pc_a, pc_v) ↦ₐ lw }}}
+  Axiom has_lseal : LWord -> ENum -> Prop.
+
+  Print dfrac.
+
+  Print excl.excl.
+
+  Context `{!inG Σ (gmapR nat (agreeR EId))} {mygname : gname}.
+
+  Search gmapR.
+
+  Print gmapR.
+
+  Eval compute in cmra_car (gmapR nat (agreeR EId)).
+  Definition enclave_q (e : ENum) (id : EId) : iProp Σ :=
+    own (A := gmapR nat (agreeR EId)) mygname (empty : gmap nat _).
+
+  (* TODO @Denis *)
+  Lemma wp_estoreid E pc_p pc_b pc_e pc_a pc_v lw rs1 rs2 rd seal p b e a v any x :
+    decodeInstrWL lw = EStoreId rs1 rs2 rd →
+    isCorrectLPC (LCap pc_p pc_b pc_e pc_a pc_v) →
+    writeAllowed p →
+    {{{ PC ↦ᵣ LCap pc_p pc_b pc_e pc_a pc_v
+        ∗ (pc_a, pc_v) ↦ₐ lw
+        ∗ rs1 ↦ᵣ seal
+        ∗ rs2 ↦ᵣ LCap p b e a v
+        ∗ rd ↦ᵣ any
+        ∗ (a, v) ↦ₐ x }}}
       Instr Executable @ E
-    {{{ RET FailedV; PC ↦ᵣ LCap pc_p pc_b pc_e pc_a pc_v ∗ (pc_a, pc_v) ↦ₐ lw }}}.
+    {{{ retv, RET retv;
+        (pc_a, pc_v) ↦ₐ lw
+        (* something with the pc increment *)
+        ∗ rs1 ↦ᵣ seal
+        ∗ rs2 ↦ᵣ LCap p b e a v
+        ∗ (
+          ⌜ retv = NextIV ⌝
+          ∗ rd ↦ᵣ (LWInt 1)
+          ∗ ∃ (id : EId), ∃ (enum : ENum),
+            (a, v) ↦ₐ (LWInt id)
+            ∗ (enclave_q enum id)
+            ∗ ⌜ has_lseal seal enum ⌝
+        ) ∨ (
+          ⌜ retv = FailedV ⌝
+          ∗ rd ↦ᵣ any
+          ∗ (a, v) ↦ₐ x
+        )
+
+    }}}.
   Proof.
-   (*  iIntros (Hinstr Hvpc φ) "[Hpc Hpca] Hφ". *)
-   (*  apply isCorrectLPC_isCorrectPC_iff in Hvpc; cbn in Hvpc. *)
-   (*  iApply wp_lift_atomic_head_step_no_fork; auto. *)
-   (*  iIntros (σ1 ns l1 l2 nt) "Hσ1 /=". destruct σ1; simpl. *)
-   (*  iDestruct "Hσ1" as (lr lm vmap) "(Hr & Hm & %HLinv)"; simpl in HLinv. *)
-   (*  iDestruct (@gen_heap_valid with "Hr Hpc") as %?. *)
-   (*  iDestruct (@gen_heap_valid with "Hm Hpca") as %?. *)
-   (*  iModIntro. *)
-   (*  iSplitR. by iPureIntro; apply normal_always_head_reducible. *)
-   (*  iIntros (e2 σ2 efs Hstep). *)
-   (*  apply prim_step_exec_inv in Hstep as (-> & -> & (c & -> & Hstep)). *)
-   (*  iNext; iIntros "_". *)
-   (*  iSplitR; auto. eapply step_exec_inv in Hstep; eauto. *)
-   (*  2: rewrite -/((lword_get_word (LCap pc_p pc_b pc_e pc_a pc_v))) *)
-   (*  ; eapply state_corresponds_reg_get_word ; eauto. *)
-   (*  2: eapply state_corresponds_mem_correct_PC ; eauto; cbn ; eauto. *)
-   (*  cbn in Hstep; simplify_eq. *)
-   (*  iModIntro. *)
-   (*  iSplitR "Hφ Hpc Hpca"; last (iApply "Hφ" ; iFrame). *)
+    iIntros (Hinstr Hvpc Hwa φ) "(Hpc & Hpca & Hrs1 & Hrs2 & Hrd & Ha) Hφ".
+    apply isCorrectLPC_isCorrectPC_iff in Hvpc; cbn in Hvpc.
+    iApply wp_lift_atomic_head_step_no_fork; auto.
+    iIntros (σ1 ns l1 l2 nt) "Hσ1 /=". destruct σ1; simpl.
+    iDestruct "Hσ1" as (lr lm vmap) "(Hr & Hm & %HLinv)"; simpl in HLinv.
+    iDestruct (@gen_heap_valid with "Hr Hpc") as %?.
+    iDestruct (@gen_heap_valid with "Hm Hpca") as %?.
+    iModIntro.
+    iSplitR. by iPureIntro; apply normal_always_head_reducible.
+    iIntros (e2 σ2 efs Hstep).
+    apply prim_step_exec_inv in Hstep as (-> & -> & (c & -> & Hstep)).
+    iNext; iIntros "_".
+    iSplitR; auto. eapply step_exec_inv in Hstep; eauto.
+    2: rewrite -/((lword_get_word (LCap pc_p pc_b pc_e pc_a pc_v)))
+    ; eapply state_corresponds_reg_get_word ; eauto.
+    2: eapply state_corresponds_mem_correct_PC ; eauto; cbn ; eauto.
+    cbn in Hstep; simplify_eq.
+    iModIntro.
+    (* iSplitR "Hφ Hpc Hpca". last (iApply "Hφ" ; iFrame). *)
    (*  iExists lr, lm, vmap. *)
    (*  iFrame; auto. *)
    (* Qed. *)
